src/program_proof/rsm/distx/invariance/commit.v
@@ -1,17 +1,396 @@
 From Perennial.program_proof.rsm.distx Require Import prelude.
 
-Lemma resm_to_tmods_lookup_Some resm ts wrs :
-  resm_to_tmods resm !! ts = Some wrs ->
+Lemma lookup_resm_to_tmods_Some resm ts wrs :
+  resm_to_tmods resm !! ts = Some wrs ↔
   resm !! ts = Some (ResCommitted wrs).
 Proof.
-  intros Hresm.
-  rewrite /resm_to_tmods lookup_omap in Hresm.
+  rewrite /resm_to_tmods lookup_omap.
   destruct (resm !! ts) as [res |] eqn:Hres; last done.
-  by destruct res as [wrsx |] eqn:Hwrsx; first inv Hresm.
+  split; intros Hresm.
+  - by destruct res as [wrsx |] eqn:Hwrsx; first inv Hresm.
+  - by rewrite Hresm /=.
 Qed.
+
+Lemma lookup_resm_to_tmods_None resm ts :
+  resm_to_tmods resm !! ts = None ↔
+  resm !! ts = None ∨ resm !! ts = Some ResAborted.
+Proof.
+  split; intros Hresm.
+  - destruct (resm !! ts) as [res |] eqn:Hres; last by left.
+    destruct res as [wrs |]; last by right.
+    exfalso.
+    by rewrite /resm_to_tmods lookup_omap Hres in Hresm.
+  - rewrite /resm_to_tmods lookup_omap.
+    by destruct Hresm as [Hresm | Hresm]; rewrite Hresm.
+Qed.
+
+Lemma conflict_free_head_commit future tmods ts wrs1 wrs2 :
+  head future = Some (ActCmt ts wrs1) ->
+  tmods !! ts = Some wrs2 ->
+  conflict_free future tmods ->
+  wrs2 = wrs1.
+Admitted.
+
+Lemma conflict_free_le_all future tmods ts wrs :
+  head future = Some (ActCmt ts wrs) ->
+  conflict_free future tmods ->
+  le_all ts (dom tmods).
+Admitted.
+
+Lemma ext_by_lnrz_inv_commit ts v cmtd lnrz kmodl :
+  kmodl !! ts = Some v ->
+  le_all ts (dom kmodl) ->
+  ext_by_lnrz cmtd lnrz kmodl ->
+  ext_by_lnrz (last_extend ts cmtd ++ [v]) lnrz (delete ts kmodl).
+Proof.
+  intros Hv Hles Hext.
+  destruct Hext as (vlast & Hprefix & Hlast & Hlen & Hext).
+  (* Obtain [length cmtd ≤ ts < length lnrz]. *)
+  apply elem_of_dom_2 in Hv as Hts.
+  apply Hlen in Hts.
+  exists v.
+  split.
+  { (* Re-establish prefix. *)
+    apply prefix_pointwise.
+    intros i Hi.
+    (* Obtain [i < S ts]. *)
+    rewrite last_length last_extend_length_eq_n in Hi; [| set_solver | lia].
+    destruct (decide (i < length cmtd)%nat) as [Hilt | Hige].
+    { (* Case: before extension [i < length cmtd]. *)
+      rewrite /last_extend Hlast /extend.
+      rewrite -app_assoc lookup_app_l; last done.
+      by apply prefix_lookup_lt.
+    }
+    rewrite Nat.nlt_ge in Hige.
+    assert (is_Some (lnrz !! i)) as [u Hu].
+    { rewrite lookup_lt_is_Some. lia. }
+    assert (Higeweak : (pred (length cmtd) ≤ i)%nat) by lia.
+    rewrite Hu.
+    destruct (decide (i < ts)%nat) as [Hits | Hits].
+    { (* Case: read-extension [i < ts]. *)
+      specialize (Hext _ _ Higeweak Hu).
+      rewrite lookup_app_l; last first.
+      { by rewrite last_extend_length_eq_n; [| set_solver | lia]. }
+      rewrite /last_extend Hlast /extend.
+      rewrite lookup_app_r; last done.
+      rewrite lookup_replicate.
+      split; last lia.
+      rewrite -Hext.
+      apply prev_dbval_lt_all.
+      intros n Hn.
+      (* Obtain [ts ≤ n]. *)
+      specialize (Hles _ Hn). simpl in Hles.
+      (* Prove [i < n] by [i < ts] and [ts ≤ n]. *)
+      lia.
+    }
+    (* Case: write-extension [i = ts]. *)
+    assert (i = ts) by lia. clear Hits Hi. subst i.
+    rewrite lookup_snoc_Some. right.
+    split.
+    { by rewrite last_extend_length_eq_n; [| set_solver | lia]. }
+    specialize (Hext _ _ Higeweak Hu).
+    by rewrite (prev_dbval_lookup _ _ _ _ Hv) in Hext.
+  }
+  split.
+  { (* Re-establish last. *)
+    by rewrite last_snoc.
+  }
+  split.
+  { (* Re-establish len. *)
+    intros n Hn.
+    rewrite last_length last_extend_length_eq_n; [| set_solver | lia].
+    rewrite dom_delete_L elem_of_difference not_elem_of_singleton in Hn.
+    destruct Hn as [Hin Hne].
+    specialize (Hlen _ Hin). simpl in Hlen.
+    specialize (Hles _ Hin). simpl in Hles.
+    lia.
+  }
+  (* Re-establish ext. *)
+  intros t u Ht Hu.
+  rewrite last_length last_extend_length_eq_n in Ht; [| set_solver | lia].
+  erewrite prev_dbval_delete; [| lia | done | done].
+  apply Hext; [lia | done].
+Qed.
+
+Lemma ext_by_cmtd_inv_commit repl cmtd kmodc ts v :
+  ts ≠ O ->
+  kmodc !! ts = None ->
+  ext_by_cmtd repl cmtd kmodc ts ->
+  ext_by_cmtd repl (last_extend ts cmtd ++ [v]) (<[ts := v]> kmodc) ts.
+Proof.
+  intros Hnz Hts Hext.
+  rewrite /ext_by_cmtd Hts in Hext.
+  destruct Hext as [[tsr Hext] Hlen].
+  rewrite /ext_by_cmtd lookup_insert Hext last_extend_twice.
+  destruct (decide (cmtd = [])) as [-> | Hnnil]; first done.
+  do 2 f_equal.
+  assert (tsr ≤ ts)%nat; last lia.
+  specialize (Hlen Hnz).
+  rewrite Hext in Hlen.
+  etrans; last apply Hlen.
+  by apply last_extend_length_ge_n.
+Qed.
+
+Lemma lnrz_txns_destined_inv_commit tids tmodcs tmodas resm ts wrs :
+  ts ∈ dom tmodcs ->
+  ts ∉ dom (resm_to_tmods resm) ->
+  lnrz_txns_destined tids tmodcs tmodas resm ->
+  lnrz_txns_destined tids (delete ts tmodcs) tmodas (<[ts:=ResCommitted wrs]> resm).
+Proof.
+  rewrite /lnrz_txns_destined.
+  intros Htsin Htsnotin Hdst tsx Htsx.
+  clear Htsin Htsnotin.
+  specialize (Hdst _ Htsx). simpl in Hdst.
+  rewrite dom_delete_L resm_to_tmods_insert_committed dom_insert_L.
+  destruct Hdst as [[Hin Hnotin] | Hdst].
+  { left. set_solver. }
+  destruct Hdst as [[Hin Hnotin] | [Hin Hnotin]].
+  { right. left.
+    split; first done.
+    admit.
+  }
+  destruct (decide (tsx = ts)) as [-> | Hne].
+  { left. set_solver. }
+  right. right. set_solver.
+Admitted.
 
 Section inv.
   Context `{!distx_ghostG Σ}.
+
+  Lemma kmod_lnrz_update {γ k kmod1 kmod2} kmod :
+    kmod_lnrz_half γ k kmod1 -∗
+    kmod_lnrz_half γ k kmod2 ==∗
+    kmod_lnrz_half γ k kmod ∗ kmod_lnrz_half γ k kmod.
+  Admitted.
+
+  Lemma kmod_lnrz_big_agree {γ keys kmods f} :
+    dom kmods = keys ->
+    ([∗ set] k ∈ keys, kmod_lnrz_half γ k (f k)) -∗
+    ([∗ map] k ↦ kmod ∈ kmods, kmod_lnrz_half γ k kmod) -∗
+    ⌜map_Forall (λ k kmod, kmod = f k) kmods⌝.
+  Proof.
+    iIntros (Hdom) "Hkeys Hkmods".
+    rewrite -Hdom.
+    rewrite big_sepS_big_sepM.
+    iCombine "Hkmods Hkeys" as "Hkmods".
+    rewrite -big_sepM_sep.
+    iApply big_sepM_pure.
+    iApply (big_sepM_impl with "Hkmods").
+    iIntros "!>" (k kmod Hkmod) "[Hkmod Hf]".
+    iApply (kmod_lnrz_agree with "Hf Hkmod").
+  Qed.
+
+  Lemma kmod_lnrz_big_agree_update {γ keys kmods f} f' :
+    dom kmods = keys ->
+    ([∗ set] k ∈ keys, kmod_lnrz_half γ k (f k)) -∗
+    ([∗ map] k ↦ kmod ∈ kmods, kmod_lnrz_half γ k kmod) ==∗
+    ([∗ set] k ∈ keys, kmod_lnrz_half γ k (f' k)) ∗
+    ([∗ map] k ↦ kmod ∈ kmods, kmod_lnrz_half γ k (f' k) ∗ ⌜kmod = f k⌝).
+  Proof.
+    iIntros (Hdom) "Hkeys Hkmods".
+    rewrite -Hdom.
+    rewrite 2!big_sepS_big_sepM.
+    iCombine "Hkmods Hkeys" as "Hkmods".
+    rewrite -2!big_sepM_sep.
+    iAssert (⌜map_Forall (λ k kmod, kmod = f k) kmods⌝)%I as %Heq.
+    { iApply big_sepM_pure.
+      iApply (big_sepM_impl with "Hkmods").
+      iIntros "!>" (k kmod Hkmod) "[Hkmod Hf]".
+      iApply (kmod_lnrz_agree with "Hf Hkmod").
+    }
+    iApply big_sepM_bupd.
+    iApply (big_sepM_mono with "Hkmods").
+    iIntros (k kmod Hkmod) "[Hkmod Hf]".
+    iMod (kmod_lnrz_update (f' k) with "Hkmod Hf") as "[Hkmod Hf]".
+    iFrame.
+    iPureIntro.
+    by specialize (Heq _ _ Hkmod).
+  Qed.
+
+  Lemma kmod_cmtd_update {γ k kmod1 kmod2} kmod :
+    kmod_cmtd_half γ k kmod1 -∗
+    kmod_cmtd_half γ k kmod2 ==∗
+    kmod_cmtd_half γ k kmod ∗ kmod_cmtd_half γ k kmod.
+  Admitted.
+
+  Lemma kmod_cmtd_big_agree {γ keys kmods f} :
+    dom kmods = keys ->
+    ([∗ set] k ∈ keys, kmod_cmtd_half γ k (f k)) -∗
+    ([∗ map] k ↦ kmod ∈ kmods, kmod_cmtd_half γ k kmod) -∗
+    ⌜map_Forall (λ k kmod, kmod = f k) kmods⌝.
+  Proof.
+    iIntros (Hdom) "Hkeys Hkmods".
+    rewrite -Hdom.
+    rewrite big_sepS_big_sepM.
+    iCombine "Hkmods Hkeys" as "Hkmods".
+    rewrite -big_sepM_sep.
+    iApply big_sepM_pure.
+    iApply (big_sepM_impl with "Hkmods").
+    iIntros "!>" (k kmod Hkmod) "[Hkmod Hf]".
+    iApply (kmod_cmtd_agree with "Hf Hkmod").
+  Qed.
+
+  (* TODO: separate agree from update *)
+  Lemma kmod_cmtd_big_agree_update {γ keys kmods f} f' :
+    dom kmods = keys ->
+    ([∗ set] k ∈ keys, kmod_cmtd_half γ k (f k)) -∗
+    ([∗ map] k ↦ kmod ∈ kmods, kmod_cmtd_half γ k kmod) ==∗
+    ([∗ set] k ∈ keys, kmod_cmtd_half γ k (f' k)) ∗
+    ([∗ map] k ↦ kmod ∈ kmods, kmod_cmtd_half γ k (f' k) ∗ ⌜kmod = f k⌝).
+  Proof.
+    iIntros (Hdom) "Hkeys Hkmods".
+    rewrite -Hdom.
+    rewrite 2!big_sepS_big_sepM.
+    iCombine "Hkmods Hkeys" as "Hkmods".
+    rewrite -2!big_sepM_sep.
+    iAssert (⌜map_Forall (λ k kmod, kmod = f k) kmods⌝)%I as %Heq.
+    { iApply big_sepM_pure.
+      iApply (big_sepM_impl with "Hkmods").
+      iIntros "!>" (k kmod Hkmod) "[Hkmod Hf]".
+      iApply (kmod_cmtd_agree with "Hf Hkmod").
+    }
+    iApply big_sepM_bupd.
+    iApply (big_sepM_mono with "Hkmods").
+    iIntros (k kmod Hkmod) "[Hkmod Hf]".
+    iMod (kmod_cmtd_update (f' k) with "Hkmod Hf") as "[Hkmod Hf]".
+    iFrame.
+    iPureIntro.
+    by specialize (Heq _ _ Hkmod).
+  Qed.
+
+  Lemma keys_inv_prepared_at_ts γ resm kmodls kmodcs wrs ts :
+    dom wrs = dom kmodls ->
+    resm !! ts = None ->
+    all_prepared γ ts wrs -∗
+    ([∗ map] key ↦ kmodl;kmodc ∈ kmodls;kmodcs,
+       key_inv_no_kmodl_kmodc γ key kmodl kmodc) -∗
+    txnres_auth γ resm -∗
+    ([∗ set] gid ∈ gids_all, group_inv γ gid) -∗
+    ([∗ map] key ↦ kmodl;kmodc ∈ kmodls;kmodcs,
+       key_inv_with_tsprep_no_kmodl_kmodc γ key ts kmodl kmodc) ∗
+    txnres_auth γ resm ∗
+    ([∗ set] gid ∈ gids_all, group_inv γ gid).
+  Proof.
+    iIntros (Hdom Hnone) "#Hpreps Hkeys Hresm Hgroups".
+    iApply (big_sepM2_impl_res with "Hkeys [Hresm Hgroups]").
+    { iFrame. }
+    iIntros (k kmodl kmodc Hkmodl Hkmodc) "!> Hkey [Hresm Hgroups]".
+    assert (Hinwrs : k ∈ dom wrs).
+    { by rewrite Hdom elem_of_dom. }
+    iDestruct "Hpreps" as "[Hwrs Hpreps]".
+    set gid := key_to_group k.
+    iDestruct (big_sepS_elem_of _ _ gid with "Hpreps") as "Hprep".
+    { by apply elem_of_ptgroups. }
+    iDestruct (big_sepS_elem_of_acc _ _ gid with "Hgroups") as "[Hgroup HgroupsC]".
+    { apply elem_of_key_to_group. }
+    do 2 iNamed "Hgroup".
+    iDestruct (txnprep_lookup with "Hpm Hprep") as %Hp.
+    assert (is_Some (stm !! ts)) as [res Hres].
+    { rewrite -elem_of_dom. apply elem_of_dom_2 in Hp. set_solver. }
+    destruct res as [pwrs | |]; last first.
+    { (* Case: Txn [ts] has already aborted. Contradiction. *)
+      iDestruct ("Htks" $! log stm tpls with "[] []") as "Htk"; [done | done |].
+      iDestruct (big_sepM_lookup with "Htk") as "Htkabt"; first apply Hres.
+      iDestruct (txnres_lookup with "Hresm Htkabt") as %Habt.
+      congruence.
+    }
+    { (* Case: Txn [ts] has already committed. Contradiction. *)
+      iDestruct ("Htks" $! log stm tpls with "[] []") as "Htk"; [done | done |].
+      iDestruct (big_sepM_lookup with "Htk") as "Htkcmt"; first apply Hres.
+      iDestruct "Htkcmt" as (wrs') "Htkcmt".
+      iDestruct (txnres_lookup with "Hresm Htkcmt") as %Hcmt.
+      congruence.
+    }
+    iDestruct (big_sepM_lookup with "Hvp") as "Hpwrs"; first apply Hres.
+    iDestruct "Hpwrs" as (wrs') "(Hwrs' & _ & %Hvw & %Hne & %Hpwrs)".
+    iDestruct (txnwrs_receipt_agree with "Hwrs Hwrs'") as %->.
+    assert (Hinpwrs : k ∈ dom pwrs).
+    { rewrite Hpwrs /wrs_group.
+      assert (Hgoal : k ∈ filter (λ k, key_to_group k = gid) (dom wrs)).
+      { by rewrite elem_of_filter. }
+      by rewrite filter_dom_L in Hgoal.
+    }
+    assert (is_Some (tpls !! k)) as [tpl Htpl].
+    { pose proof (apply_cmds_dom _ _ _ Hrsm) as Hdomtpls.
+      rewrite -elem_of_dom Hdomtpls.
+      rewrite /valid_wrs in Hvw.
+      (* solved with [Hinwrs] and [Hvw] *)
+      set_solver.
+    }
+    iAssert (⌜Forall (λ c, valid_pts_of_command c) log⌝)%I as %Hvpts.
+    { rewrite Forall_forall.
+      iIntros (x Hx).
+      iDestruct (log_cpool_incl with "Hlog Hcpool") as %Hsubsume.
+      rewrite /cpool_subsume_log Forall_forall in Hsubsume.
+      specialize (Hsubsume _ Hx).
+      iDestruct (big_sepS_elem_of with "Hvc") as "Hc"; first apply Hsubsume.
+      destruct x; [done | | done | done]. simpl.
+      by iDestruct "Hc" as (?) "(_ & %Hvts & _)".
+    }
+    pose proof (pts_consistency _ Hvpts) as Hpts.
+    specialize (Hpts _ _ _ _ _ _ Hrsm Hres Htpl Hinpwrs).
+    (* Take [tuple_repl_half] from [Hrepls]. *)
+    iDestruct (big_sepM_lookup_acc _ _ k tpl with "Hrepls") as "[[Hhist Hts] HreplsC]".
+    { by rewrite /tpls_group map_lookup_filter_Some. }
+    iDestruct (key_inv_no_kmodl_kmodc_unseal_tsprep with "Hkey") as (tsprep) "Hkey".
+    (* Finally, deduce [tsprep = ts]. *)
+    iAssert (⌜tsprep = ts⌝)%I as %->.
+    { iNamed "Hkey".
+      iDestruct (ts_repl_agree with "Htsprep Hts") as %Heq.
+      by rewrite Hpts in Heq.
+    }
+    iDestruct ("HreplsC" with "[$Hhist $Hts]") as "Hrepls".
+    iDestruct ("HgroupsC" with "[-Hresm Hkey]") as "Hgroups".
+    { iFrame "∗ # %". }
+    iFrame.
+  Qed.
+
+  Definition key_inv_after_commit
+    γ (key : dbkey) (tsprep : nat) (kmodl kmodc : dbkmod) : iProp Σ :=
+    ∃ v, let kmodl' := delete tsprep kmodl in
+         let kmodc' := <[tsprep := v]> kmodc in
+         key_inv_with_tsprep_no_kmodl_kmodc γ key tsprep kmodl' kmodc' ∗
+         ⌜kmodl !! tsprep = Some v⌝.
+
+  Lemma key_inv_commit γ kmodl kmodc ts k v :
+    ts ≠ O ->
+    le_all ts (dom kmodl) ->
+    kmodl !! ts = Some v ->
+    kmodc !! ts = None ->
+    key_inv_with_tsprep_no_kmodl_kmodc γ k ts kmodl kmodc -∗
+    key_inv_with_tsprep_no_kmodl_kmodc γ k ts (delete ts kmodl) (<[ts:=v]> kmodc).
+  Proof.
+    iIntros (Hnz Hles Hkmodl Hkmodc) "Hkey".
+    iNamed "Hkey".
+    iNamed "Hprop".
+    pose proof (ext_by_lnrz_inv_commit _ _ _ _ _ Hkmodl Hles Hdiffl) as Hdiffl'.
+    pose proof (ext_by_cmtd_inv_commit _ _ _ _ v Hnz Hkmodc Hdiffc) as Hdiffc'.
+    iFrame "∗ # %".
+    iPureIntro.
+    by rewrite lookup_insert_ne.
+  Qed.
+
+  Lemma keys_inv_commit γ kmodls kmodcs ts :
+    ts ≠ O ->
+    map_Forall (λ _ kmodl, le_all ts (dom kmodl)) kmodls ->
+    map_Forall (λ _ kmodl, is_Some (kmodl !! ts)) kmodls ->
+    map_Forall (λ _ kmodc, kmodc !! ts = None) kmodcs ->
+    ([∗ map] key ↦ kmodl;kmodc ∈ kmodls;kmodcs,
+       key_inv_with_tsprep_no_kmodl_kmodc γ key ts kmodl kmodc) -∗
+    ([∗ map] key ↦ kmodl;kmodc ∈ kmodls;kmodcs,
+       key_inv_after_commit γ key ts kmodl kmodc).
+  Proof.
+    iIntros (Hnz Hles Hkmodls Hkmodcs) "Hkeys".
+    iApply (big_sepM2_impl with "Hkeys").
+    iIntros (k kmodl kmodc Hkmodl Hkmodc) "!> Hkey".
+    specialize (Hkmodls _ _ Hkmodl). simpl in Hkmodls.
+    specialize (Hles _ _ Hkmodl). simpl in Hles.
+    specialize (Hkmodcs _ _ Hkmodc). simpl in Hkmodcs.
+    destruct Hkmodls as [v Hv].
+    iExists v.
+    iSplit; last done.
+    by iApply key_inv_commit.
+  Qed.
 
   (**
    * The commit action modifies the following logical states in [txn_inv]:
@@ -45,20 +424,22 @@ Section inv.
     txns_lnrz_receipt γ tid -∗
     all_prepared γ tid wrs -∗
     txn_inv_no_future γ future -∗
+    ([∗ set] gid ∈ gids_all, group_inv γ gid) -∗
     ([∗ set] key ∈ keys_all, key_inv γ key) ==∗
     txn_inv_no_future γ (tail future) ∗
+    ([∗ set] gid ∈ gids_all, group_inv γ gid) ∗
     ([∗ set] key ∈ keys_all, key_inv γ key) ∗
     txnres_cmt γ tid wrs.
   Proof.
-    iIntros (Hhead) "#Htid #Hprep Htxnsys Hkeys".
+    iIntros (Hhead) "#Htid #Hprep Htxnsys Hgroups Hkeys".
     iNamed "Htxnsys".
     iDestruct (txns_lnrz_elem_of with "Htxnsl Htid") as %Htid.
     apply Hdest in Htid as Hcases.
-    destruct Hcases as [[Hin Hnotin] | Hcases].
+    destruct Hcases as [[Hresm Hnotin] | Hcases].
     { (* Case: Txn [tid] has already aborted or committed. *)
-      rewrite elem_of_dom in Hin.
-      destruct Hin as [wrsc Hwrs].
-      apply resm_to_tmods_lookup_Some in Hwrs.
+      rewrite elem_of_dom in Hresm.
+      destruct Hresm as [wrsc Hwrs].
+      rewrite lookup_resm_to_tmods_Some in Hwrs.
       iDestruct (big_sepM_lookup with "Hvr") as "#Hres"; first apply Hwrs.
       iAssert (⌜wrsc = wrs⌝)%I as %->.
       { iDestruct "Hres" as "[Hwrsc _]".
@@ -84,6 +465,170 @@ Section inv.
       additional premise. *)
       admit.
     }
+    (* Case: Txn [tid] predicted to commit. Update states and extract commitment witness. *)
+    (* Obtain [resm !! ts = None]. *)
+    rewrite not_elem_of_dom lookup_resm_to_tmods_None in Hnotin.
+    destruct Hnotin as [Hnone | Habt]; last first.
+    { iDestruct (big_sepM_lookup with "Hvr") as "Habt"; first apply Habt.
+      iDestruct (all_prepared_some_aborted_false with "Hprep Habt") as %[].
+    }
+    (* Obtain [wrsx], the write set in the result map of [tid]. *)
+    rewrite elem_of_dom in Htmodcs.
+    destruct Htmodcs as [wrsx Hwrs].
+    (* Obtain eq of write set between the predicted [wrs] and the [wrsx] in the result map. *)
+    pose proof (conflict_free_head_commit _ _ _ _ _ Hhead Hwrs Hcf). subst wrsx.
+    assert (Hdom : dom wrs ⊆ keys_all) by admit.
+    (* Take [dom wrs] of [kmod_lnrz_half] and [kmod_cmtd_half]. *)
+    iDestruct (big_sepS_subseteq_difference_1 _ _ (dom wrs) with "Hkmodls") as "[Hkmodls HkmodlsO]".
+    { apply Hdom. }
+    iDestruct (big_sepS_subseteq_difference_1 _ _ (dom wrs) with "Hkmodcs") as "[Hkmodcs HkmodcsO]".
+    { apply Hdom. }
+    (* Take [dom wrs] of [key_inv]. *)
+    iDestruct (big_sepS_subseteq_acc _ _ (dom wrs) with "Hkeys") as "[Hkeys HkeysC]".
+    { apply Hdom. }
+    (* Extract [kmod_lnrz_half] and [kmod_cmtd_half] out of [key_inv]. *)
+    iDestruct (keys_inv_extract_kmodl_kmodc with "Hkeys") as "Hkeys".
+    iDestruct "Hkeys" as (kmodls kmodcs) "(Hkeys & Hkmodls' & Hkmodcs' & %Hdomkmodls)".
+    iDestruct (big_sepM2_dom with "Hkeys") as %Hdomkmodcs.
+    rewrite Hdomkmodls in Hdomkmodcs. symmetry in Hdomkmodcs.
+    (* Agreement of [kmod_lnrz_half] and [kmod_cmtd_half] between [txn_inv] and [key_inv]. *)
+    iDestruct (kmod_lnrz_big_agree with "Hkmodls Hkmodls'") as %Hkmodls.
+    { apply Hdomkmodls. }
+    iDestruct (kmod_cmtd_big_agree with "Hkmodcs Hkmodcs'") as %Hkmodcs.
+    { apply Hdomkmodcs. }
+    (* Agreement and update of [kmod_lnrz_half] and [kmod_cmtd_half]. *)
+    set tmodcs' := delete tid tmodcs.
+    iMod (kmod_lnrz_big_agree_update (λ k, vslice tmodcs' k) with
+           "Hkmodls Hkmodls'") as "[Hkmodls Hkmodls']".
+    { apply Hdomkmodls. }
+    iAssert ([∗ map] k ↦ kmod ∈ kmodls, kmod_lnrz_half γ k (delete tid kmod))%I
+      with "[Hkmodls']" as "Hkmodls'".
+    { iApply (big_sepM_impl with "Hkmodls'").
+      iIntros (k kmod Hkmod) "!> [Hkmods %Heq]".
+      subst tmodcs'.
+      by rewrite vslice_delete Heq.
+    }
+    set resm' := <[tid := ResCommitted wrs]> resm.
+    iMod (kmod_cmtd_big_agree_update (λ k, vslice (resm_to_tmods resm') k) with "Hkmodcs Hkmodcs'")
+      as "[Hkmodcs Hkmodcs']".
+    { apply Hdomkmodcs. }
+    iAssert ([∗ map] k ↦ kmod; v ∈ kmodcs; wrs, kmod_cmtd_half γ k (<[tid := v]> kmod))%I
+      with "[Hkmodcs']" as "Hkmodcs'".
+    { iApply (big_sepM_sepM2_impl with "Hkmodcs'"); first done.
+      iIntros (k kmod v Hkmod Hv) "!> [Hkmods %Heq]".
+      subst resm'.
+      by rewrite resm_to_tmods_insert_committed (vslice_insert_Some _ _ _ _ _ Hv) Heq.
+    }
+    (* Prove that for all [key ∈ dom wrs], the lock must be currently granted to [tid]. *)
+    iDestruct (keys_inv_prepared_at_ts with "Hprep Hkeys Hresm Hgroups")
+      as "(Hkeys & Hresm & Hgroups)"; [done | done |].
+    (* Prove for each [kmodl] and [kmodc], [is_Some (kmodl !! tid)] and [kmodc !! tid = None]. *)
+    assert (Hkmodlstid : map_Forall (λ _ kmodl, is_Some (kmodl !! tid)) kmodls).
+    { intros k kmodl Hkmodl.
+      specialize (Hkmodls _ _ Hkmodl). simpl in Hkmodls.
+      rewrite Hkmodls lookup_vslice /dual_lookup Hwrs.
+      rewrite -elem_of_dom.
+      apply elem_of_dom_2 in Hkmodl.
+      set_solver.
+    }
+    assert (Hkmodcstid : map_Forall (λ _ kmodc, kmodc !! tid = None) kmodcs).
+    { intros k kmodc Hkmodc.
+      specialize (Hkmodcs _ _ Hkmodc). simpl in Hkmodcs.
+      rewrite Hkmodcs lookup_vslice /dual_lookup.
+      assert (Hresm : resm_to_tmods resm !! tid = None).
+      { rewrite lookup_resm_to_tmods_None. by left. }
+      by rewrite Hresm.
+    }
+    (* Re-establish [key_inv] w.r.t. commit. *)
+    iDestruct (keys_inv_commit with "Hkeys") as "Hkeys".
+    { by eapply Hnz, elem_of_dom_2. }
+    { intros k kmodl Hkmodl.
+      pose proof (conflict_free_le_all _ _ _ _ Hhead Hcf) as Hle.
+      specialize (Hkmodls _ _ Hkmodl). simpl in Hkmodls.
+      eapply set_Forall_subseteq; last apply Hle.
+      rewrite Hkmodls.
+      apply dom_vslice_subseteq.
+    }
+    { apply Hkmodlstid. }
+    { apply Hkmodcstid. }
+    iAssert ([∗ map] k ↦ kmodl;kmodc ∈ kmodls; kmodcs,
+               ∃ v, kmod_cmtd_half γ k (<[tid := v]> kmodc) ∗ ⌜kmodl !! tid = Some v⌝)%I
+      with "[Hkmodcs']" as "Hkmodcs'".
+    { rewrite 2!big_sepM2_alt.
+      iDestruct "Hkmodcs'" as "[_ Hkmodcs]".
+      iSplit; first by rewrite Hdomkmodls Hdomkmodcs.
+      iApply (big_sepM_impl_dom_eq with "Hkmodcs").
+      { rewrite 2!dom_map_zip_with_L. set_solver. }
+      iIntros (k kmodcv kmodlc Hkmodcv Hkmodlc) "!> Hkmodcv".
+      destruct kmodcv as [kmodc v]. destruct kmodlc as [kmodl kmodc'].
+      rewrite map_lookup_zip_Some in Hkmodcv. destruct Hkmodcv as [Hkmodc Hv].
+      rewrite map_lookup_zip_Some in Hkmodlc. destruct Hkmodlc as [Hkmodl Hkmodc'].
+      rewrite Hkmodc in Hkmodc'. symmetry in Hkmodc'. inv Hkmodc'.
+      iFrame.
+      iPureIntro.
+      simpl.
+      specialize (Hkmodls _ _ Hkmodl). simpl in Hkmodls.
+      by rewrite Hkmodls lookup_vslice /dual_lookup Hwrs.
+    }
+    iAssert ([∗ set] k ∈ dom wrs, key_inv γ k)%I with "[Hkmodls' Hkmodcs' Hkeys]" as "Hkeys".
+    { iDestruct (big_sepM_big_sepM2_1 _ _ kmodcs with "Hkmodls'") as "Hkmodls'".
+      { by rewrite Hdomkmodls Hdomkmodcs. }
+      iCombine "Hkmodls' Hkmodcs'" as "Hkmods".
+      rewrite -big_sepM2_sep.
+      iCombine "Hkeys Hkmods" as "Hkeys".
+      rewrite -big_sepM2_sep.
+      rewrite big_sepS_big_sepM.
+      iApply (big_sepM2_sepM_impl with "Hkeys"); first done.
+      iIntros (k kmodl kmodc v Hkmodl Hkmodc Hv) "!> (Hkey & Hkmodl & Hkmodc)".
+      clear Hv v.
+      iDestruct "Hkmodc" as (v) "[Hkmodc %Hv]".
+      iDestruct "Hkey" as (v') "[Hkey %Hv']".
+      rewrite Hv in Hv'. symmetry in Hv'. inv Hv'.
+      iNamed "Hkey".
+      iFrame "∗ #".
+    }
+    iDestruct ("HkeysC" with "Hkeys") as "Hkeys".
+    (* Update the unmodified part of [kmod_lnrz_half]. *)
+    iAssert ([∗ set] x ∈ (keys_all ∖ dom wrs), kmod_lnrz_half γ x (vslice tmodcs' x))%I
+      with "[HkmodlsO]" as "HkmodlsO".
+    { iApply (big_sepS_impl with "HkmodlsO").
+      iIntros (k Hk) "!> Hkmod".
+      subst tmodcs'.
+      assert (Hnotinwrs : wrs !! k = None).
+      { rewrite -not_elem_of_dom. set_solver. }
+      by rewrite (vslice_delete_None _ _ _ _ Hwrs Hnotinwrs).
+    }
+    (* Update the unmodified part of [kmod_cmtd_half]. *)
+    iAssert ([∗ set] x ∈ (keys_all ∖ dom wrs), kmod_cmtd_half γ x (vslice (resm_to_tmods resm') x))%I
+      with "[HkmodcsO]" as "HkmodcsO".
+    { iApply (big_sepS_impl with "HkmodcsO").
+      iIntros (k Hk) "!> Hkmod".
+      subst resm'.
+      rewrite resm_to_tmods_insert_committed.
+      assert (Hnotinwrs : wrs !! k = None).
+      { rewrite -not_elem_of_dom. set_solver. }
+      rewrite (vslice_insert_None _ _ _ _ _ Hnotinwrs); last first.
+      { rewrite lookup_resm_to_tmods_None. by left. }
+      done.
+    }
+    (* Combine the modified and unmodified parts of [kmod_lnrz_half] and [kmod_cmtd_half]. *)
+    iDestruct (big_sepS_subseteq_difference_2 with "Hkmodls HkmodlsO") as "Hkmodls".
+    { apply Hdom. }
+    iDestruct (big_sepS_subseteq_difference_2 with "Hkmodcs HkmodcsO") as "Hkmodcs".
+    { apply Hdom. }
+    (* Add [(tid, ResCommitted wrs)] to [resm] and extract a witness. *)
+    iMod (txnres_insert _ (ResCommitted wrs) with "Hresm") as "Hresm"; first apply Hnone.
+    iDestruct (txnres_witness _ _ tid with "Hresm") as "#Hcmt".
+    { by rewrite lookup_insert. }
+    (* Re-establish [valid_res]. *)
+    (* Re-establish [conflict_free] and [conflict_past]. *)
+    pose proof (conflict_free_inv_commit _ _ _ _ Hhead Hcf) as Hcf'.
+    pose proof (conflict_past_inv_commit _ _ _ _ _ Hhead Hcp) as Hcp'.
+    iFrame "∗ # %".
+    iModIntro.
+    iSplit.
+    { by iApply (big_sepM_insert_2 with "[Hprep] Hvr"). }
+    
   Admitted.
 
 End inv.
