src/program_proof/rsm/distx/prelude.v
@@ -2,6 +2,6 @@ From Perennial.program_proof Require Export grove_prelude.
 From Perennial.program_logic Require Export atomic. (* prefer the ncfupd atomics *)
 From Perennial.program_proof.rsm Require Export big_sep.
 From Perennial.program_proof.rsm.pure Require Export
-  dual_lookup extend fin_maps largest_before list misc nonexpanding_merge vslice word.
+  dual_lookup extend fin_maps largest_before list misc nat nonexpanding_merge sets vslice word.
 From Perennial.program_proof.rsm.distx Require Export
   base cmd res inv.
