src/program_proof/rsm/pure/nat.v
@@ -1,0 +1,19 @@
+From iris.proofmode Require Import proofmode.
+
+Definition lt_all (n : nat) (ns : gset nat) :=
+  set_Forall (λ x, n < x)%nat ns.
+
+Definition le_all (n : nat) (ns : gset nat) :=
+  set_Forall (λ x, n ≤ x)%nat ns.
+
+Definition gt_all (n : nat) (ns : gset nat) :=
+  set_Forall (λ x, x < n)%nat ns.
+
+Definition ge_all (n : nat) (ns : gset nat) :=
+  set_Forall (λ x, x ≤ n)%nat ns.
+
+Definition nz_all (ns : gset nat) :=
+  set_Forall (λ x, x ≠ O) ns.
+
+Definition outside_all (ub lb : nat) (ns : gset nat) :=
+  set_Forall (λ x, x ≤ ub ∨ lb < x)%nat ns.
